linux/proofs/early_alloc/generated_spec.v
@@ -18,7 +18,7 @@ Section spec.
   (* Specifications for function [clear_page]. *)
   Definition type_of_clear_page :=
     fn(∀ p : loc; (p @ (&own (uninit (PAGE_LAYOUT)))); True)
-      → ∃ () : (), (void); (p ◁ₗ (uninit (PAGE_LAYOUT))).
+      → ∃ () : (), (void); (p ◁ₗ (zeroed (PAGE_LAYOUT))).
 
   (* Function [hyp_early_alloc_page] has been skipped. *)
 
@@ -27,8 +27,11 @@ Section spec.
   (* Specifications for function [hyp_early_alloc_page1]. *)
   Definition type_of_hyp_early_alloc_page1 :=
     fn(∀ n : nat; (ptr); (global_with_type "cur1" Own (&own (uninit (ly_set_size PAGE_LAYOUT n)))) ∗ (global_with_type "size1" Own (n @ int u64)))
-      → ∃ m : nat, (optionalO (λ _ : unit,   &own (uninit (PAGE_LAYOUT))
+      → ∃ m : nat, (optionalO (λ _ : unit,   &own (zeroed (PAGE_LAYOUT))
       ) (null)); (global_with_type "size1" Own (m @ int u64)) ∗ (global_with_type "cur1" Own (&own (uninit (ly_set_size PAGE_LAYOUT m)))).
 
-  (* Function [hyp_early_alloc_init1] has been skipped. *)
+  (* Specifications for function [hyp_early_alloc_init1]. *)
+  Definition type_of_hyp_early_alloc_init1 :=
+    fn(∀ n : nat; (&own (uninit (ly_set_size PAGE_LAYOUT n))), (n @ (int (u64))); (global_with_type "cur1" Own (uninit LPtr)) ∗ (global_with_type "size1" Own (uninit u64)) ∗ (global_with_type "base1" Own (uninit LPtr)))
+      → ∃ m : nat, (void); (global_with_type "size1" Own (m @ int u64)) ∗ (global_with_type "cur1" Own (&own (uninit (ly_set_size PAGE_LAYOUT m)))) ∗ (global_with_type "base1" Own (uninit LPtr)).
 End spec.
