linux/proofs/early_alloc/generated_proof_hyp_early_alloc_init1.v
@@ -1,1 +1,28 @@
-(* You were too lazy to even write a spec for this function. *)
+From refinedc.typing Require Import typing.
+From refinedc.linux.early_alloc Require Import generated_code.
+From refinedc.linux.early_alloc Require Import generated_spec.
+Set Default Proof Using "Type".
+
+(* Generated from [linux/early_alloc.c]. *)
+Section proof_hyp_early_alloc_init1.
+  Context `{!typeG Σ} `{!globalG Σ}.
+
+  (* Typing proof for [hyp_early_alloc_init1]. *)
+  Lemma type_hyp_early_alloc_init1 (base1 cur1 size1 : loc) :
+    global_locs !! "base1" = Some base1 →
+    global_locs !! "cur1" = Some cur1 →
+    global_locs !! "size1" = Some size1 →
+    ⊢ typed_function (impl_hyp_early_alloc_init1 base1 cur1 size1) type_of_hyp_early_alloc_init1.
+  Proof.
+    start_function "hyp_early_alloc_init1" (n) => arg_virt arg_size.
+    split_blocks ((
+      ∅
+    )%I : gmap label (iProp Σ)) ((
+      ∅
+    )%I : gmap label (iProp Σ)).
+    - repeat liRStep; liShow.
+      all: print_typesystem_goal "hyp_early_alloc_init1" "#0".
+    Unshelve. all: sidecond_hook; prepare_sideconditions; normalize_and_simpl_goal; try solve_goal; unsolved_sidecond_hook.
+    all: print_sidecondition_goal "hyp_early_alloc_init1".
+  Qed.
+End proof_hyp_early_alloc_init1.
